Merge hint experiments

tactics/prolog.v
@@ -29,16 +29,118 @@ Elpi Accumulate lp:{{
   }}. 
 Elpi Typecheck.
 
+Elpi Db hints.db lp:{{ 
+  type hint term -> term -> prop.
+}}.
+
+Elpi Command print_db.
+Elpi Accumulate Db hints.db.
+Elpi Accumulate lp:{{
+  main [] :- std.findall (hint Term_ Type_) L, !, coq.say "The Db contains" L.
+}}.
+
+Elpi Command add_db.
+Elpi Accumulate Db hints.db.
+Elpi Accumulate lp:{{
+  main [trm Term] :-
+    coq.typecheck Term Type ok,
+    % coq.say "Type" Type,
+    coq.elpi.accumulate _ "hints.db" (clause _ _ (hint Term Type)).
+}}.
+Elpi Typecheck.
+
+Elpi Tactic dprolog.
+Elpi Accumulate File "pbt/dep-kernel.mod".
+Elpi Accumulate File "pbt/fpc-qbound.mod".
+Elpi Accumulate File "pbt/fpc-pair.mod".
+Elpi Accumulate Db hints.db.
 
 
  Elpi Query interp {{lp:G = lp:G}}.
  Elpi Bound Steps 1000000.
+Inductive insert (x:nat) : list nat -> list nat -> Prop :=
+(* i_n : insert x [] [x] *)
+ i_s : forall y: nat, forall ys: list nat, x <= y -> insert x (y :: ys) (x :: y :: ys)
+| i_c : forall y: nat, forall ys: list nat, forall rs: list nat,  y<=x -> insert x ys rs -> insert x (y :: ys) (y :: rs).
+
+Axiom InsAx : forall x, insert x [] [x].
+
+Elpi add_db (InsAx).
+Elpi print_db.
+
+(* Elpi Trace. *)
+Goal exists l, insert 1 [] l.
+eexists.
+elpi dprolog 10.
+Show Proof.
+Qed.
+
+Module test.
+Theorem help: forall n m, m <= n -> n > m.
+Admitted.
+
 
 Inductive insert (x:nat) : list nat -> list nat -> Prop :=
-i_n : insert x [] [x]
-| i_s : forall y: nat, forall ys: list nat, x <= y -> insert x (y :: ys) (x :: y :: ys)
-| i_c : forall y: nat, forall ys: list nat, forall rs: list nat,  insert x ys rs -> insert x (y :: ys) (y :: rs).
+ i_n : insert x [] [x] 
+| i_s : forall y: nat, forall ys: list nat, y > x -> insert x (y :: ys) (x :: y :: ys)
+| i_c : forall y: nat, forall ys: list nat, forall rs: list nat,  y<=x -> insert x ys rs -> insert x (y :: ys) (y :: rs).
+
+End test.
+
+Elpi add_db (test.help).
+Goal exists l, test.insert 3 [1;4;8] l.
+eexists.
+
+elpi dprolog 10.
 
 Goal insert 1 [] [1].
 elpi dprolog 10.
 Qed.
+Lemma i1:  exists R, insert 2 [0;1] R.
+elpi  dprolog 10.
+Qed.
+Lemma i2:  exists R, insert 2 [0;1] R.
+eexists.
+apply i_c.
+apply i_c.
+apply i_n.
+Qed.
+Print i2.
+Print le.
+ Inductive ordered : list nat -> Prop :=
+onl : ordered []
+| oss : forall x : nat, ordered [x]
+| ocn : forall (x y : nat) (l : list nat),
+     ordered (y :: l) -> x <= y -> ordered (x :: y :: l).
+
+Goal exists Xs, ordered Xs.
+eexists.
+elpi prolog  3.
+apply onl.
+Restart.
+eexists.
+elpi dprolog 10.
+Qed.
+
+ Goal ordered [0;1;2;6].
+   elpi prolog  10.
+   Fail elpi prolog size 10.
+
+   elpi dprolog 20.
+   Qed.
+
+   Inductive append : list nat -> list nat -> list nat -> Prop :=
+   anl : forall xs, append [] xs xs
+   |acn : forall xs ys zs x, 
+        append xs ys zs -> append (x :: xs) ys (x :: zs).
+
+  (* Goal exists L1 L2, append L1 L2 [0;1;2;6]. *)
+  Goal append  [0] [1;2;6] [0;1;2;6].
+  elpi dprolog 20.
+Qed.
+
+Goal exists L, append  L [1;2;6] [0;1;2;6].
+ eexists.
+ elpi dprolog 20.
+Qed.
+
